# Exam 2019

## Task 1

1. False F
2. True T
3. False F
4. True T
5. False T
6. True F
7. False T
8. False F
9. True T
10. True T

## Task 2

FOL:

$$
\begin{aligned}
&R_1: \forall x \ [\forall y \ [Animal(y) \implies Loves(x, y)]] \implies [\exists z \ Loves(z, x)] \\
&R_2: \forall x \ [\exists y \ (Animal(y) \wedge Kills(x, y))] \implies \neg (\exists z \ Loves(z, x)) \\
&R_3: \forall x \ [Animal(x) \implies Loves(Sofie, x)] \\
&R_4: Kills(Sofie, Kismet) \vee Kills(CarAccident, Kismet) \\
&R_5: Cat(Kismet)
\end{aligned}
$$

The query is Did CarAccident kill Kismet.

1 ) Conversion to CNF. $R_4$ and $R_5$ are already in CNF. First we replace every implication with the propositional equvilant:

$$
\begin{aligned}
&R_1: \forall x \ \neg [\forall y \ [\neg Animal(y) \vee Loves(x, y)]] \vee [\exists z \ Loves(z, x)] \\
&R_2: \forall x \ \neg [\exists y \ (Animal(y) \wedge Kills(x, y))] \vee \neg (\exists z \ Loves(z, x)) \\
&R_3: \forall x \ [\neg Animal(x) \vee Loves(Sofie, x)] \\
\end{aligned}
$$

We then move the negation inwards, using De Morgans Rule:

$$
\begin{aligned}
&R_1: \forall x \ [\exists y \ \neg [\neg Animal(y) \vee Loves(x, y)]] \vee [\exists z \ Loves(z, x)] \\
&R_2: \forall x \ [\forall y \ \neg (Animal(y) \wedge Kills(x, y))] \vee (\forall z \ \neg Loves(z, x)) \\
&R_3: \forall x \ [\neg Animal(x) \vee Loves(Sofie, x)] \\
\end{aligned}
$$

$$
\begin{aligned}
&R_1: \forall x \ [\exists y \ [Animal(y) \wedge \neg Loves(x, y)]] \vee [\exists z \ Loves(z, x)] \\
&R_2: \forall x \ [\forall y \ (\neg Animal(y) \vee \neg Kills(x, y))] \vee (\forall z \ \neg Loves(z, x)) \\
&R_3: \forall x \ [\neg Animal(x) \vee Loves(Sofie, x)] \\
\end{aligned}
$$

We then perform existential instansiation to remove the existential quantifier (this only applies to $R_1$):

$$
\begin{aligned}
&R_1: \forall x \ [Animal(F(x)) \wedge \neg Loves(x, F(x))] \vee Loves(G(x), x)
\end{aligned}
$$

Then we can remove the universal quantifier:

$$
\begin{aligned}
&R_1: [Animal(F(x)) \wedge \neg Loves(x, F(x))] \vee Loves(G(x), x) \\
&R_2: (\neg Animal(y) \vee \neg Kills(x, y)) \vee \neg Loves(z, x) \\
&R_3: \neg Animal(x) \vee Loves(Sofie, x) \\
\end{aligned}
$$

Lastly, we distribute so that we can a conjunction of literals.

$$
\begin{aligned}
&R_1: (Animal(F(x)) \vee Loves(G(x), x)) \wedge (\neg Loves(x, F(x)) \vee Loves(G(x), x))\\
&R_2: \neg Animal(y) \vee \neg Kills(x, y) \vee \neg Loves(z, x) \\
&R_3: \neg Animal(x) \vee Loves(Sofie, x) \\
\end{aligned}
$$

For ease, we split $R_1$:

$$
\begin{aligned}
&R_{1,1}: Animal(F(x)) \vee Loves(G(x), x) \\
&R_{1,2}: \neg Loves(x, F(x)) \vee Loves(G(x), x)
\end{aligned}
$$

The negated goal in CNF is:

$$
\begin{aligned}
&\neg Kills(CarAccident, Kismet)
\end{aligned}
$$

2 ) There is not much extra we have to know. However, we need to assume that all cats are animals. This gives the rule:

$$
R_6: \forall x \ Cat(x) \implies Animal(x)
$$

Which in CNF becomes

$$
R_6: \neg Cat(x) \vee Animal(x)
$$

3 ) We know have everything we need to perform the proof by resolution.

First we assume CarAccident did not kill Kismet. We know that either Sofie or CarAccident killed Kismet, so we can resolve with $Kills(Sofie, Kismet)$.

We then use $R_5$ and $R_6$ to resolve that Kismet is indeed an animal. For $R_6$ we need to unify with the substitution $\theta = \{x/Kismet\}$
We then get $\neg Cat(Kismet) \vee Animal(Kismet) \vee Cat(Kismet)$ which resolves to $Animal(Kismet)$.

Then we use $R_2$:

$\neg Animal(y) \vee \neg Kills(x, y) \vee \neg Loves(z, x) \vee Animal(Kismet)$

With the substitution $\theta = \{y/Kismet\}$ resolves with
$\neg Kills(x, y) \vee \neg Loves(z, x)$

However we have infered that Sofie killed Kismet so we get:

$\neg Kills(Sofie, Kismet) \vee \neg Loves(z, Sofie) \vee Kills(Sofie, Kismet)$

Using the substitution $\theta = \{x/Sofie,\ y/Kismet\}$, which resolves to $\neg Loves(z, Sofie)$

Sofie loves all animals, we get using $R_3$ and $R_{1,2}$:
$\neg Animal(x) \vee Loves(Sofie, x) \vee \neg Loves(z, F(z)) \vee Loves(G(z), z)$

Using the substitution $\theta = \{z/Sofie, x/F(Sofie)\}$ resolves with

$\neg Animal(x) \vee Loves(G(Sofie), Sofie)$

Then using $R_{1,1}$:

$Animal(F(x)) \vee Loves(G(x), x) \vee \neg Animal(F(Sofie)) \vee Loves(G(Sofie), Sofie)$

and using $\theta = \{x/Sofie\}$ it resolves to $Loves(G(Sofie), Sofie)$

This means that both someone loves Sofie and noone loves Sofie, which is a contradiction. This means that we have proved that it was indeed CarAccident that killed Kismet.

## Task 3

1 ) A* expands the node with the least f value, where $f = g + h$. This gives the following expansion, assumed it uses the given pseudo-code:

A - C - B - D - G

2 ) It would return [A, C, G] as the path, which in this case is not the optimal solution. C is first expanded with a f value of 6. When B is expanded, it notices that C's f value is actually 5, but because C already is in the closed list, it does not update it.

3 ) The main issue with the algorithm is that it does not allow for the reexpansion of nodes. This can be done by removing the "not in closed" and only adding to the frontier if it has a lower g value:

```pseudo
add N to CLOSED
FOR all children M of N:
    if N.g + cost(N, M) < M.g:
        M.g = N.g + cost(N, M)
        M.parent = N
        M.h = heuristic(M)
        ADD M to FRONTIER
ENDFOR
```

4 ) It depends whether or not the graph contains loops with negative cycles, as you would always lower the g value and therefore the f value. It migth also happend that the negative cycle is far away from the goal, so A* never reaches near the cycle, in which case it would find the optimal solution. However it would not find it for every case.

## Task 4

1 ) For 1 it is {R}, for 2 it is {G, B}, for 3 it is {G, B}, for 4 it is {R, G, B} and for 5 it is {R, B}

2 )

1R - 2R - 2G - 3R - 3G - 3B - 4R - 5R - 5B - 4G - 4B - 2B - 3R - 3G - 4R - 5R - 5B

3 )
Forward checking works in the way that whenever we assign a value to a variable, we make the variable arc-consistent, that is for every unassigned variable that is connected to the newly assigned variable through a constraint, we delete from this variables domain values that is not consistent with the value chosen for our original variable.

4 )
1R - 2G - 3B - 4R - 2B - 3G - 4R - 5B

## Task 5

1 ) For agent1 we notice that u_1(H, G) > u_1(NH, G) and that u_1(H, NG) > u_1(NH, NG). This means that action H dominates over action NG, and is a dominated strategy for agent1. Notice for agent2 that u_2(H, G) < u_2(H, NG) but u_2(NH, G) > u_2(NH, NG). Agent2 therefore has none dominated strategy.

2 ) (H, NG) is a nash equilibrium, which gives the utility values (3, 1).

3 ) (NH, G) and (H, G) are Pareto optimal joint actions.

4 ) A socail welfare maximazing joint is also pareto optimal because available utility is not wasted. Utility is maximized and if you were to change solution, one or the other would have to yield utilty, either to the other or completely lost.

## Task 6

1 ) A list

* e(E) = 6 - 5 = 1
* e(F) = 5 - 5 = 0
* e(G) = 6 - 5 = 1
* e(H) = 5 - 5 = 0
* e(I) = 4 - 5 = -1

* e(J) = 5 - 6 = -1
* e(K) = 5 - 5 = 0
* e(L) = 5 - 5 = 0
* e(M) = 6 - 6 = 0
* e(N) = 4 - 6 = -2

* e(O) = 5 - 4 = 1
* e(P) = 6 - 4 = 2

2 ) Yes

A = 1, B = -1, C = -1, D = 2

3 ) It will prune K, L, M and N.

## Task 7

1 ) Simple-reflex-agents have no notion of goals, so I'm unsure what the question really asks. I guess you can use obtain the current state by interpreting the percept, and then make an action based on the state.

2 ) By constructing the truth table, the statement is false for P = False and Q = True. The statement is therefore satisfiable since it's true for some models.

3 ) "Any person who has an umbrella is not wet" can be translated to:
$\forall x: (Person(x) \wedge HasUmbrella(x)) \implies \neg Wet(x)$

4 ) "John has at least two daughters" is translated to
$\exists x, y \ Daughter(x, John) \wedge Daughter(y, John) \wedge \neg (x = y)$

5 ) A hill-climbing algorithm tries to find the global maximum. One can alter the heuristic function, such that in fact finds the global minimum, by for example giving minimum values higher values in the heuristic function.

6 ) No, it will not be admissible, for example if you are at the last step in a graph with 10 action layers, i.e the state in layer 9, the heuristic function would yield 10 as the heuristic value, which grossly overestimates the actual cost to the goal.

7 ) action1 > action2 >Â action3, i.e first action1 then action2 and lastly action3.

8 ) Regression planning works in a backwards manner, starting from the goal and asking what should I do to reach this state.

9 )

Student:

* birthYear: number
* age: currentYear - birthYear

10 ) There are multiple versions of that environment so its hard to say. I would say it's episodic, since it does not care about earlier state, and makes each action independtantly of each other action. It's stochastic since we are dealing with probablitites, i.e we don't know for certain that cleaning a tile will result in that tile being clean. The environment is still static, there are no external factors that the agent has to deal with.
